Solved efficiency problems for Applicative/Monad instances for parsers by moving proofs to separate lemmas. Removed lots of useless code. Refactored MonadJoin and MonadComp. They are now subclasses of Applicative.

Instances/Cont.v
@@ -16,20 +16,14 @@ Instance FunctorCont (R : Type) : Functor (Cont R) :=
 }.
 Proof. all: reflexivity. Defined.
 
-Definition ret_Cont {R A : Type} (a : A) : Cont R A :=
+Definition ret_Cont
+  {R A : Type} (a : A) : Cont R A :=
     fun f : A -> R => f a.
 
 Definition ap_Cont
   {R A B : Type} (f : Cont R (A -> B)) (x : Cont R A) : Cont R B :=
     fun y : B -> R => f (fun h : A -> B => x (fun a : A => y (h a))).
-(*
-Proof.
-  unfold Cont in *. intro y. apply f. intro h. apply x. intro a.
-    apply y. apply h. assumption. Show Proof.
 
- apply y. apply h.
-    fun br : B -> R => ca (fun a : A => cf (fun ab : A -> B => br (ab a))).
-*)
 Instance ApplicativeCont (R : Type) : Applicative (Cont R) :=
 {
     is_functor := FunctorCont R;
@@ -38,11 +32,17 @@ Instance ApplicativeCont (R : Type) : Applicative (Cont R) :=
 }.
 Proof. all: reflexivity. Defined.
 
-Definition join_Cont {R A : Type} (cca : Cont R (Cont R A)) : Cont R A :=
+Definition join_Cont
+  {R A : Type} (cca : Cont R (Cont R A)) : Cont R A :=
     fun f : A -> R => cca (fun g : (A -> R) -> R => g f).
 
-Definition bind_Cont {R A B : Type} (ca : Cont R A) (f : A -> Cont R B)
-    : Cont R B := fun g : B -> R => ca (fun x : A => f x g).
+Definition bind_Cont
+  {R A B : Type} (ca : Cont R A) (f : A -> Cont R B) : Cont R B :=
+    fun g : B -> R => ca (fun x : A => f x g).
+
+Definition compM_Cont
+  {R A B C : Type} (f : A -> Cont R B) (g : B -> Cont R C) (a : A)
+    : Cont R C := fun y : C -> R => f a (fun b : B => g b y).
 
 Theorem Cont_not_Alternative :
   (forall R : Type, Alternative (Cont R)) -> False.
