MonadBind/Monad.v
@@ -1,8 +1,6 @@
-Add Rec LoadPath "/home/Zeimer/Code/Coq".
+Add Rec LoadPath "/home/zeimer/Code/Coq".
 
-Require Export HSLib.Base.
-Require Import HSLib.Instances.ListInst.
-
+Require Import HSLib.Base.
 Require Export HSLib.Functor.Functor.
 Require Export HSLib.Applicative.Applicative.
 
@@ -11,14 +9,18 @@ Class Monad (M : Type -> Type) : Type :=
 {
     is_applicative :> Applicative M;
     bind : forall {A B : Type}, M A -> (A -> M B) -> M B;
-    bind_ret_l : forall (A B : Type) (f : A -> M B) (a : A),
-      bind (ret a) f = f a;
-    bind_ret_r : forall (A : Type) (ma : M A),
-      bind ma ret = ma;
-    assoc : forall (A B C : Type) (ma : M A) (f : A -> M B) (g : B -> M C),
-      bind (bind ma f) g = bind ma (fun x => bind (f x) g);
-    bind_fmap : forall (A B C : Type) (f : A -> B) (x : M A) (g : B -> M C),
-      bind (fmap f x) g = bind x (f .> g);
+    bind_ret_l :
+      forall (A B : Type) (f : A -> M B) (a : A),
+        bind (ret a) f = f a;
+    bind_ret_r :
+      forall (A : Type) (ma : M A),
+        bind ma ret = ma;
+    assoc :
+      forall (A B C : Type) (ma : M A) (f : A -> M B) (g : B -> M C),
+        bind (bind ma f) g = bind ma (fun x => bind (f x) g);
+    bind_fmap :
+      forall (A B C : Type) (f : A -> B) (x : M A) (g : B -> M C),
+        bind (fmap f x) g = bind x (f .> g);
     fmap_bind :
       forall (A B C : Type) (x : M A) (f : A -> M B) (g : B -> C),
         fmap g (bind x f) = bind x (fun x0 : A => fmap g (f x0));
@@ -78,83 +80,11 @@ repeat (monad'; repeat match goal with
     | |- context [match ?x with _ => _ end] => destruct x
 end; monad'); try (unfold compose, id; cbn; congruence; fail).
 
-(*Section Lifts.
-
-Variable M : Type -> Type.
-Variable inst : Monad M.
-Variables A B C D E F : Type.
-
-Definition liftM2
-  (f : A -> B -> C)
-  (ma : M A) (mb : M B) : M C :=
-  ma >>= fun a : A =>
-  mb >>= fun b : B => ret (f a b).
-
-Definition liftM3
-  (f : A -> B -> C -> D)
-  (ma : M A) (mb : M B) (mc : M C) : M D :=
-  ma >>= fun a : A =>
-  mb >>= fun b : B => 
-  mc >>= fun c : C => ret (f a b c).
-
-Definition liftM4
-  (f : A -> B -> C -> D -> E)
-  (ma : M A) (mb : M B) (mc : M C) (md : M D) : M E :=
-  ma >>= fun a : A =>
-  mb >>= fun b : B =>
-  mc >>= fun c : C =>
-  md >>= fun d : D => ret (f a b c d).
-
-Definition liftM5
-  (f : A -> B -> C -> D -> E -> F)
-  (ma : M A) (mb : M B) (mc : M C) (md : M D) (me : M E) : M F :=
-  ma >>= fun a : A =>
-  mb >>= fun b : B =>
-  mc >>= fun c : C =>
-  md >>= fun d : D =>
-  me >>= fun e : E => ret (f a b c d e).
-
-End Lifts.
-
-Arguments liftM2 [M inst A B C] _ _ _.
-Arguments liftM3 [M inst A B C D] _ _ _ _.
-Arguments liftM4 [M inst A B C D E] _ _ _ _ _.
-Arguments liftM5 [M inst A B C D E F] _ _ _ _ _ _.*)
-
 Section MonadicFuns.
 
 Variable M : Type -> Type.
 Variable inst : Monad M.
 Variables A B C D E F : Type.
-
-(*Fixpoint filterM (f : A -> M bool) (la : list A) : M (list A) :=
-match la with
-    | [] => ret []
-    | h :: t => f h >>= fun b : bool => if b
-        then liftM2 (@cons A) (ret h) (filterM f t)
-        else filterM f t
-end.
-
-Fixpoint sequence
-    (lma : list (M A)) : M (list A) :=
-match lma with
-    | [] => ret []
-    | h :: t => liftM2 (@cons A) h (sequence t)
-end.
-
-Fixpoint replicateM (n : nat) (ma : M A) : M (list A) :=
-match n with
-    | 0 => ret []
-    | S n' => liftM2 (@cons A) ma (replicateM n' ma)
-end.
-
-Fixpoint zipWithM (f : A -> B -> M C)
-    (la : list A) (lb : list B) : M (list C) :=
-match la, lb with
-    | [], _ => ret []
-    | _, [] => ret []
-    | ha :: ta, hb :: tb => liftM2 (@cons C) (f ha hb) (zipWithM f ta tb)
-end.*)
 
 Fixpoint foldM (f : A -> B -> M A) (dflt : A) (l : list B)
     : M A :=
@@ -163,41 +93,9 @@ match l with
     | h :: t => f dflt h >>= fun a : A => foldM f a t
 end.
 
-(*Definition when (b : bool) (mu : M unit) : M unit :=
-match b with
-    | true => mu
-    | false => ret tt
-end.
-
-Definition unless (b : bool) (mu : M unit) : M unit :=
-    when (negb b) mu.*)
-
 End MonadicFuns.
 
-(*Arguments filterM [M] [inst] [A] _ _.
-Arguments sequence [M] [inst] [A] _.
-Arguments replicateM [M] [inst] [A] _ _.
-Arguments zipWithM [M] [inst] [A] [B] [C] _ _ _.*)
 Arguments foldM [M] [inst] [A] [B] _ _ _.
-(*Arguments when [M] [inst] _ _.
-Arguments unless [M] [inst] _ _.*)
-
-(*Section MonadicFuns2.
-
-Variable M : Type -> Type.
-Variable inst : Monad M.
-Variables A B C D E F : Type.
-
-Definition mapM (f : A -> M B) (la : list A) : M (list B) :=
-  sequence (fmap f la).
-
-Definition forM (la : list A) (f : A -> M B) : M (list B) :=
-  mapM f la.
-
-End MonadicFuns2.
-
-Arguments mapM [M] [inst] [A] [B] _ _.
-Arguments forM [M] [inst] [A] [B] _ _.*)
 
 Section DerivedLaws.
 
@@ -209,49 +107,47 @@ Theorem compM_assoc :
   forall (A B C D : Type) (f : A -> M B) (g : B -> M C) (h : C -> M D),
     f >=> (g >=> h) = (f >=> g) >=> h.
 Proof.
-  intros. unfold compM. ext a. rewrite assoc. reflexivity.
+  unfold compM. monad.
 Qed.
 
 Theorem compM_id_left :
   forall (A B : Type) (f : A -> M B), ret >=> f = f.
 Proof.
-  intros. unfold compM. ext a. apply bind_ret_l.
+  unfold compM. monad.
 Qed.
 
 Theorem compM_id_right :
   forall (A B : Type) (f : A -> M B), f >=> ret = f.
 Proof.
-  intros. unfold compM. ext a. apply bind_ret_r.
+  unfold compM. monad.
 Qed.
 
 Theorem bind_compM :
   forall (A B : Type) (ma : M A) (f : A -> M B),
     bind ma f = ((fun _ : unit => ma) >=> f) tt.
 Proof.
-  intros. unfold compM. reflexivity.
+  unfold compM. reflexivity.
 Qed.
 
 Theorem bind_join_fmap :
   forall (A B C : Type) (ma : M A) (f : A -> M B),
     bind ma f = join (fmap f ma).
 Proof.
-  intros. unfold join. rewrite bind_fmap. reflexivity.
+  unfold join. monad.
 Qed.
 
 Theorem join_fmap :
   forall (A : Type) (x : M (M (M A))),
     join (fmap join x) = join (join x).
 Proof.
-  intros. unfold join. rewrite bind_fmap, assoc. reflexivity.
+  unfold join. monad.
 Qed.
 
 Theorem join_ret :
   forall (A : Type) (x : M A),
     join (ret x) = join (fmap ret x).
 Proof.
-  intros. unfold join.
-  rewrite bind_ret_l, bind_fmap, id_right, bind_ret_r.
-  reflexivity.
+  unfold join. monad.
 Qed.
 
 End DerivedLaws.
