MonadComp/Monad.v
@@ -1,15 +1,13 @@
-Add Rec LoadPath "/home/Zeimer/Code/Coq".
+Add Rec LoadPath "/home/zeimer/Code/Coq".
 
 Require Import HSLib.Base.
-Require Import HSLib.Instances.ListInst.
-
-Require Import HSLib.Functor.Functor.
+Require Export HSLib.Functor.Functor.
+Require Export HSLib.Applicative.Applicative.
 
 (* Definition of monad using ret and monadic composition. *)
 Class Monad (M : Type -> Type) : Type :=
 {
-    is_functor :> Functor M;
-    ret : forall {A : Type}, A -> M A;
+    is_applicative :> Applicative M;
     compM : forall {A B C : Type}, (A -> M B) -> (B -> M C) -> (A -> M C);
     compM_assoc : forall (A B C D : Type) (f : A -> M B) (g : B -> M C)
         (h : C -> M D), compM f (compM g h) = compM (compM f g) h;
@@ -17,11 +15,9 @@ Class Monad (M : Type -> Type) : Type :=
         compM ret g = g;
     id_right : forall (A B : Type) (f : A -> M B),
         compM f ret = f;
-    fmap_ret : forall (A B : Type) (f : A -> B) (x : A),
-      fmap f (ret x) = ret (f x)
 }.
 
-Coercion is_functor : Monad >-> Functor.
+Coercion is_applicative : Monad >-> Applicative.
 
 Definition bind
   {A B : Type} {M : Type -> Type} {_ : Monad M} (ma : M A) (f : A -> M B)
@@ -51,100 +47,11 @@ End MonadNotations.
 
 Export MonadNotations.
 
-Section Lifts.
-
-Variable M : Type -> Type.
-Variable inst : Monad M.
-Variables A B C D E F : Type.
-
-Definition liftM
-    (f : A -> B)
-    (ma : M A) : M B :=
-    ma >>= fun a : A => ret (f a).
-
-Definition liftM2
-    (f : A -> B -> C)
-    (ma : M A) (mb : M B) : M C :=
-    ma >>= fun a : A =>
-    mb >>= fun b : B => ret (f a b).
-
-Definition liftM3
-    (f : A -> B -> C -> D)
-    (ma : M A) (mb : M B) (mc : M C) : M D :=
-    ma >>= fun a : A =>
-    mb >>= fun b : B => 
-    mc >>= fun c : C => ret (f a b c).
-
-Definition liftM4
-    (f : A -> B -> C -> D -> E)
-    (ma : M A) (mb : M B) (mc : M C) (md : M D) : M E :=
-    ma >>= fun a : A =>
-    mb >>= fun b : B =>
-    mc >>= fun c : C =>
-    md >>= fun d : D => ret (f a b c d).
-
-Definition liftM5
-    (f : A -> B -> C -> D -> E -> F)
-    (ma : M A) (mb : M B) (mc : M C) (md : M D) (me : M E) : M F :=
-    ma >>= fun a : A =>
-    mb >>= fun b : B =>
-    mc >>= fun c : C =>
-    md >>= fun d : D =>
-    me >>= fun e : E => ret (f a b c d e).
-
-End Lifts.
-
-Arguments liftM [M] [inst] [A] [B] _ _.
-Arguments liftM2 [M] [inst] [A] [B] [C] _ _ _.
-Arguments liftM3 [M] [inst] [A] [B] [C] [D] _ _ _ _.
-Arguments liftM4 [M] [inst] [A] [B] [C] [D] [E] _ _ _ _ _.
-Arguments liftM5 [M] [inst] [A] [B] [C] [D] [E] [F] _ _ _ _ _ _.
-
 Section MonadicFuns.
 
 Variable M : Type -> Type.
 Variable inst : Monad M.
 Variables A B C D E F : Type.
-
-(* TODO remove after Applicative is superclass of Monad. *)
-Definition ap (mf : M (A -> B)) (ma : M A) : M B :=
-    mf >>= fun f =>
-    ma >>= fun a => ret (f a).
-
-Fixpoint filterM (f : A -> M bool) (la : list A) : M (list A) :=
-match la with
-    | [] => ret []
-    | h :: t => f h >>= fun b : bool => if b
-        then liftM2 (@cons A) (ret h) (filterM f t)
-        else filterM f t
-end.
-
-Fixpoint sequence {M : Type -> Type} {_xd : Monad M} {A : Type}
-    (lma : list (M A)) : M (list A) :=
-match lma with
-    | [] => ret []
-    | h :: t => liftM2 (@cons A) h (sequence t)
-end.
-
-Fixpoint replicateM {A : Type} (n : nat) (ma : M A) : M (list A) :=
-match n with
-    | 0 => ret []
-    | S n' => liftM2 (@cons A) ma (replicateM n' ma)
-end.
-
-Definition mapM {A B : Type} (f : A -> M B) : list A -> M (list B) :=
-    fmap f .> sequence.
-
-Definition forM {A B : Type} (la : list A) (f : A -> M B) : M (list B) :=
-    mapM f la.
-
-Fixpoint zipWithM {A B C : Type} (f : A -> B -> M C)
-    (la : list A) (lb : list B) : M (list C) :=
-match la, lb with
-    | [], _ => ret []
-    | _, [] => ret []
-    | ha :: ta, hb :: tb => liftM2 (@cons C) (f ha hb) (zipWithM f ta tb)
-end.
 
 Fixpoint foldM {A B : Type} (f : A -> B -> M A) (dflt : A) (l : list B)
     : M A :=
@@ -152,15 +59,6 @@ match l with
     | [] => ret dflt
     | h :: t => f dflt h >>= fun a : A => foldM f a t
 end.
-
-Definition when (b : bool) (mu : M unit) : M unit :=
-match b with
-    | true => mu
-    | false => ret tt
-end.
-
-Definition unless (b : bool) (mu : M unit) : M unit :=
-    when (negb b) mu.
 
 End MonadicFuns.
 
@@ -202,15 +100,15 @@ Proof.
   intros. unfold bind.
   assert (((fun _ : unit => ret x) >=> f) tt = (ret >=> f) x).
     Focus 2. rewrite H. rewrite id_left. reflexivity.
-    unfold ret, compM. destruct inst. rewrite id_left0.
+    unfold ret, compM. destruct inst.
 Admitted. (* TODO *)
 
 Theorem join_law :
   forall A : Type, fmap join .> join = join .> join (A := A).
 Proof.
   intros. unfold compose. extensionality x. unfold join.
-  unfold id. unfold bind. compute. destruct inst; destruct is_functor0. simpl.
-  f_equal. extensionality y. destruct y. simpl.
+  unfold id. unfold bind. compute. (*
+  f_equal. extensionality y. destruct y. simpl.*)
 Abort. (* TODO *)
 
 Theorem ret_law :
