MonadJoin/Monad.v
@@ -1,39 +1,37 @@
-Add Rec LoadPath "/home/Zeimer/Code/Coq".
+Add Rec LoadPath "/home/zeimer/Code/Coq".
 
 Require Import HSLib.Base.
-Require Import HSLib.Instances.ListInst.
-
 Require Export HSLib.Functor.Functor.
+Require Export HSLib.Applicative.Applicative.
 
 (* Definition of monad using ret and join. *)
 Class Monad (M : Type -> Type) : Type :=
 {
-    is_functor :> Functor M;
-    ret : forall {A : Type}, A -> M A;
+    is_applicative :> Applicative M;
     join : forall {A : Type}, M (M A) -> M A;
-    join_law : forall (X : Type),
+    join_law :
+      forall (X : Type),
         fmap join .> join = join .> @join X;
-    ret_law : forall (X : Type),
+    ret_law :
+      forall (X : Type),
         ret .> join = fmap ret .> @join X;
-    ret_join : forall (X : Type),
-      ret .> @join X = id;
-    fmap_ret : forall (A B : Type) (f : A -> B) (x : A),
-      fmap f (ret x) = ret (f x);
     join_ret :
       forall (A : Type) (ma : M A), join (ret ma) = ma
 }.
 
-Coercion is_functor : Monad >-> Functor.
+Coercion is_applicative : Monad >-> Applicative.
 
-Definition bind {A B : Type} {M : Type -> Type} {_ : Monad M}
-    (ma : M A) (f : A -> M B) : M B :=
-    (fmap f .> join) ma.
+Definition bind
+  {A B : Type} {M : Type -> Type} {inst : Monad M} (ma : M A) (f : A -> M B)
+    : M B := (fmap f .> join) ma.
 
-Definition bind_ {M : Type -> Type} {_ : Monad M} {A B : Type}
-    (ma : M A) (mb : M B) : M B := bind ma (fun _ => mb).
+Definition bind_
+  {M : Type -> Type} {_ : Monad M} {A B : Type} (ma : M A) (mb : M B)
+    : M B := bind ma (fun _ => mb).
 
-Definition compM {A B C : Type} {M : Type -> Type} {_ : Monad M}
-    (f : A -> M B) (g : B -> M C) : A -> M C :=
+Definition compM
+  {A B C : Type} {M : Type -> Type} {inst : Monad M}
+  (f : A -> M B) (g : B -> M C) : A -> M C :=
     f .> fmap g .> join.
 
 Module MonadNotations.
@@ -54,94 +52,12 @@ End MonadNotations.
 
 Export MonadNotations.
 
-Section Lifts.
-
-Variable M : Type -> Type.
-Variable inst : Monad M.
-Variables A B C D E F : Type.
-
-Definition liftM
-    (f : A -> B)
-    (ma : M A) : M B :=
-    ma >>= fun a : A => ret (f a).
-
-Definition liftM2
-    (f : A -> B -> C)
-    (ma : M A) (mb : M B) : M C :=
-    ma >>= fun a : A =>
-    mb >>= fun b : B => ret (f a b).
-
-Definition liftM3
-    (f : A -> B -> C -> D)
-    (ma : M A) (mb : M B) (mc : M C) : M D :=
-    ma >>= fun a : A =>
-    mb >>= fun b : B => 
-    mc >>= fun c : C => ret (f a b c).
-
-Definition liftM4
-    (f : A -> B -> C -> D -> E)
-    (ma : M A) (mb : M B) (mc : M C) (md : M D) : M E :=
-    ma >>= fun a : A =>
-    mb >>= fun b : B =>
-    mc >>= fun c : C =>
-    md >>= fun d : D => ret (f a b c d).
-
-Definition liftM5
-    (f : A -> B -> C -> D -> E -> F)
-    (ma : M A) (mb : M B) (mc : M C) (md : M D) (me : M E) : M F :=
-    ma >>= fun a : A =>
-    mb >>= fun b : B =>
-    mc >>= fun c : C =>
-    md >>= fun d : D =>
-    me >>= fun e : E => ret (f a b c d e).
-
-End Lifts.
-
-Arguments liftM [M] [inst] [A] [B] _ _.
-Arguments liftM2 [M] [inst] [A] [B] [C] _ _ _.
-Arguments liftM3 [M] [inst] [A] [B] [C] [D] _ _ _ _.
-Arguments liftM4 [M] [inst] [A] [B] [C] [D] [E] _ _ _ _ _.
-Arguments liftM5 [M] [inst] [A] [B] [C] [D] [E] [F] _ _ _ _ _ _.
-
 Section MonadicFuns.
 
 Variable M : Type -> Type.
 Variable inst : Monad M.
 Variables A B C D E F : Type.
 
-(* TODO remove after Applicative is superclass of Monad. *)
-Definition ap (mf : M (A -> B)) (ma : M A) : M B :=
-    mf >>= fun f =>
-    ma >>= fun a => ret (f a).
-
-Fixpoint filterM (f : A -> M bool) (la : list A) : M (list A) :=
-match la with
-    | [] => ret []
-    | h :: t => f h >>= fun b : bool => if b
-        then liftM2 (@cons A) (ret h) (filterM f t)
-        else filterM f t
-end.
-
-Fixpoint sequence
-    (lma : list (M A)) : M (list A) :=
-match lma with
-    | [] => ret []
-    | h :: t => liftM2 (@cons A) h (sequence t)
-end.
-
-Fixpoint replicateM (n : nat) (ma : M A) : M (list A) :=
-match n with
-    | 0 => ret []
-    | S n' => liftM2 (@cons A) ma (replicateM n' ma)
-end.
-
-Fixpoint zipWithM (f : A -> B -> M C)
-    (la : list A) (lb : list B) : M (list C) :=
-match la, lb with
-    | [], _ => ret []
-    | _, [] => ret []
-    | ha :: ta, hb :: tb => liftM2 (@cons C) (f ha hb) (zipWithM f ta tb)
-end.
 
 Fixpoint foldM (f : A -> B -> M A) (dflt : A) (l : list B)
     : M A :=
@@ -150,66 +66,14 @@ match l with
     | h :: t => f dflt h >>= fun a : A => foldM f a t
 end.
 
-Definition when (b : bool) (mu : M unit) : M unit :=
-match b with
-    | true => mu
-    | false => ret tt
-end.
-
-Definition unless (b : bool) (mu : M unit) : M unit :=
-    when (negb b) mu.
-
 End MonadicFuns.
 
-Arguments ap [M] [inst] [A] [B] _ _.
-Arguments filterM [M] [inst] [A] _ _.
-Arguments sequence [M] [inst] [A] _.
-Arguments replicateM [M] [inst] [A] _ _.
-Arguments zipWithM [M] [inst] [A] [B] [C] _ _ _.
 Arguments foldM [M] [inst] [A] [B] _ _ _.
-Arguments when [M] [inst] _ _.
-Arguments unless [M] [inst] _ _.
 
-Section MonadicFuns2.
+Section DerivedLaws.
 
-Variable M : Type -> Type.
-Variable inst : Monad M.
-Variables A B C D E F : Type.
+Variables
+  (M : Type -> Type)
+  (inst : Monad M).
 
-Definition mapM (f : A -> M B) (la : list A) : M (list B) :=
-  sequence (fmap f la).
-
-Definition forM (la : list A) (f : A -> M B) : M (list B) :=
-  mapM f la.
-
-End MonadicFuns2.
-
-Arguments mapM [M] [inst] [A] [B] _ _.
-Arguments forM [M] [inst] [A] [B] _ _.
-
-(* Do notation — conflicts with the 'do' tactic combinator. *)
-
-Section MonadTheorems.
-
-Variable M : Type -> Type.
-Variable inst : Monad M.
-Variables A B C : Type.
-
-End MonadTheorems.
-
-Set Implicit Arguments.
-
-
-(*Theorem ret_bind :
-  forall (M : Type -> Type) (inst : Monad M) (A B : Type) (x : A) (f : A -> M B),
-    ret x >>= f = f x.
-Proof.
-  intros. unfold bind. rewrite join_law. unfold compose. Check fmap_ret.
-  rewrite fmap_ret.
-  pose (ret_law B). unfold compose in e.
-  change (join (ret (f x))) with ((fun x0 : M B => join (ret x0)) (f x)).
-  rewrite e.
-  pose (join_law B). unfold compose in e0.
-  assert ((fun x0 : M B => join (ret x0)) (f x) =
-  (fun x0 : M B => join (fmap ret x0)) (f x)).
-Abort. *)
+End DerivedLaws. (* TODO *)
