Misc/MonadEquiv.v
@@ -17,7 +17,9 @@ Module Comp.
 Require Import HSLib.MonadComp.Monad.
 Include HSLib.MonadComp.Monad.
 End Comp.
-(*
+
+Require Import HSLib.Applicative.Applicative.
+
 Axiom fmap_join :
   forall (M : Type -> Type) (inst : Join.Monad M) (A B : Type) (f : A -> B)
     (x : M (M A)),
@@ -30,26 +32,22 @@ Axiom fmap_pres_comp' :
 
 Instance JoinToBind (M : Type -> Type) (inst : Join.Monad M) : Bind.Monad M :=
 {
-    is_functor := @Join.is_functor M inst;
-    ret := @Join.ret M inst;
+    is_applicative := @Join.is_applicative M inst;
     bind := fun (A B : Type) (ma : M A) (f : A -> M B) =>
-        (fmap f .> Join.join) ma
+      (fmap f .> Join.join) ma
 }.
 Proof.
   all: intros.
-    unfold compose. rewrite Join.fmap_ret, Join.join_ret. reflexivity.
+    unfold compose. rewrite fmap_ret, Join.join_ret. reflexivity.
     rewrite <- Join.ret_law. unfold compose. rewrite Join.join_ret.
       reflexivity.
-    Focus 2. rewrite Join.fmap_ret. reflexivity.
     Focus 2. unfold compose. rewrite <- fmap_pres_comp'. reflexivity.
-    unfold compose. rewrite fmap_join, <- ?fmap_pres_comp'.
-Abort.
+Abort. (* TODO *)
 
 Instance BindToComp (M : Type -> Type) (inst : Bind.Monad M)
   : Comp.Monad M :=
 {
-    is_functor := @Bind.is_functor M inst;
-    ret := @Bind.ret M inst;
+    is_applicative := @Bind.is_applicative M inst;
     compM := fun (A B C : Type) (f : A -> M B) (g : B -> M C) =>
         fun a : A => Bind.bind (f a) g
 }.
@@ -58,14 +56,12 @@ Proof.
     rewrite Bind.assoc. reflexivity.
     apply Bind.bind_ret_l.
     apply Bind.bind_ret_r.
-    apply Bind.fmap_ret.
 Defined.
 
 Instance BindToJoin (M : Type -> Type) (inst : Bind.Monad M)
   : Join.Monad M :=
 {
-    is_functor := @Bind.is_functor M inst;
-    ret := @Bind.ret M inst;
+    is_applicative := @Bind.is_applicative M inst;
     join := fun (A : Type) (x : M (M A)) =>
         Bind.bind x id
 }.
@@ -75,14 +71,12 @@ Proof.
     rewrite Bind.bind_ret_l, Bind.bind_fmap, id_right, Bind.bind_ret_r.
       reflexivity.
     rewrite Bind.bind_ret_l. reflexivity.
-    rewrite Bind.fmap_ret. reflexivity.
-  rewrite Bind.bind_ret_l. reflexivity.
 Defined.
 
 Axiom comp_id :
   forall (M : Type -> Type) (inst : Comp.Monad M) (A B : Type) (f : A -> M B)
   (x : A),
-    Comp.compM id f (Comp.ret x) = f x.
+    Comp.compM id f (ret x) = f x.
 
 Axiom comp_const :
   forall (M : Type -> Type) (inst : Comp.Monad M) (A B C : Type)
@@ -92,15 +86,12 @@ Axiom comp_const :
 Instance CompToBind (M : Type -> Type) (inst : Comp.Monad M)
   : Bind.Monad M :=
 {
-    is_functor := @Comp.is_functor M inst;
-    ret := @Comp.ret M inst;
+    is_applicative := @Comp.is_applicative M inst;
     bind := fun (A B : Type) (ma : M A) (f : A -> M B) =>
       @Comp.compM M inst unit A B (fun _ => ma) f tt
 }.
 Proof.
   all: intros.
     Focus 2. rewrite Comp.id_right. reflexivity.
-    Focus 3. rewrite Comp.fmap_ret. reflexivity.
     Focus 2. rewrite comp_const.
-Abort.
-*)
+Abort. (* TODO *)
