MonadBind/MonadInst.v
@@ -6,13 +6,14 @@ Require Import HSLib.Base.
 
 Require Import HSLib.MonadBind.Monad.
 
-Require Import HSLib.Instances.Option.
-Require Import HSLib.Instances.ListInst.
-Require Import HSLib.Instances.Sum.
-Require Import HSLib.Instances.Reader.
-Require Import HSLib.Instances.Writer.
-Require Import HSLib.Instances.State.
-Require Import HSLib.Instances.Cont.
+Require Import HSLib.Instances.All.
+
+Instance MonadIdentity : Monad Identity :=
+{
+    is_applicative := Applicative_Identity;
+    bind := @bind_Identity
+}.
+Proof. all: reflexivity. Defined.
 
 Instance MonadOption : Monad option :=
 {
@@ -25,12 +26,6 @@ Proof.
       | x : option _ |- _ => destruct x
   end; cbn in *; reflexivity.
 Defined.
-
-Eval compute in (fun _ => Some 5) >=> (fun n => Some (n + 6)).
-Eval compute in Some 4 >>= fun n : nat => Some (2 * n).
-
-Eval compute in liftA2 plus (Some 2) (Some 4).
-Eval compute in liftA2 plus (Some 42) None.
 
 Lemma bind_List_app : forall (A B : Type) (l1 l2 : list A) (f : A -> list B),
     bind_List (l1 ++ l2) f = bind_List l1 f ++ bind_List l2 f.
@@ -66,24 +61,6 @@ Proof.
       rewrite IHt. reflexivity.
 Defined.
 
-Definition head {A : Type} (l : list A) : option A :=
-match l with
-    | [] => None
-    | h :: _ => Some h
-end.
-
-Fixpoint init {A : Type} (l : list A) : option (list A) :=
-match l with
-    | [] => None
-    | [_] => Some []
-    | h :: t => cons <$> ret h <*> init t
-end.
-
-Compute init [1; 2; 3].
-Compute filterA (fun _ => [true; false]) [1; 2; 3].
-Compute replicateA 3 [1; 2].
-Compute sequenceA [[1]; [2]].
-
 Instance MonadSum (A : Type) : Monad (sum A) :=
 {
     is_applicative := ApplicativeSum A;
@@ -95,11 +72,6 @@ Proof.
       | x : _ + _ |- _ => destruct x
   end; cbn in *; reflexivity.
 Defined.
-
-Eval cbn in sequenceA [inr 42; inr 5; inr 10].
-Eval cbn in sequenceA [inr 42; inr 5; inr 10; inl (fun n : nat => 2 * n)].
-
-Eval simpl in foldM (fun n m => inl (plus n m)) 0 [1; 2; 3].
 
 Instance MonadReader (R : Type) : Monad (Reader R) :=
 {
@@ -124,7 +96,7 @@ Proof.
   all: compute; intros; ext s;
   try match goal with
       | x : ?S -> _ * ?S, s : ?S |- _ => destruct (x s)
-  end; trivial.
+  end; reflexivity.
 Defined.
 
 Require Import HSLib.MonadBind.MonadState.
@@ -142,4 +114,4 @@ Instance MonadCont (R : Type) : Monad (Cont R) :=
     is_applicative := ApplicativeCont R;
     bind := @bind_Cont R
 }.
-Proof. all: trivial. Defined.
+Proof. all: reflexivity. Defined.
